opentheory/theories/group/group-thm.ml
@@ -136,6 +136,8 @@ let group_add_left_cancel_imp = prove
      ASM_REWRITE_TAC [group_add_assoc];
      MATCH_ACCEPT_TAC group_add_left_zero]]);;
 
+export_thm group_add_left_cancel_imp;;
+
 (*PARAMETRIC
 let group_add_left_cancel_imp = new_axiom
    `!x y z. group_add x y = group_add x z ==> y = z`;;
@@ -149,6 +151,8 @@ let group_add_left_cancel = prove
     DISCH_THEN SUBST1_TAC THEN
     REFL_TAC]);;
 
+export_thm group_add_left_cancel;;
+
 (*PARAMETRIC
 let group_add_left_cancel = new_axiom
    `!x y z. group_add x y = group_add x z <=> y = z`;;
@@ -160,6 +164,8 @@ let group_add_left_cancel_zero_imp = prove
    MATCH_MP_TAC group_add_left_cancel_imp THEN
    EXISTS_TAC `x : group` THEN
    ASM_REWRITE_TAC [group_add_right_zero]);;
+
+export_thm group_add_left_cancel_zero_imp;;
 
 (*PARAMETRIC
 let group_add_left_cancel_zero_imp = new_axiom
@@ -173,6 +179,8 @@ let group_add_left_cancel_zero = prove
    [MATCH_ACCEPT_TAC group_add_left_cancel_zero_imp;
     DISCH_THEN SUBST1_TAC THEN
     MATCH_ACCEPT_TAC group_add_right_zero]);;
+
+export_thm group_add_left_cancel_zero;;
 
 (*PARAMETRIC
 let group_add_left_cancel_zero = new_axiom
@@ -194,6 +202,8 @@ let group_add_right_cancel_imp = prove
      ASM_REWRITE_TAC [GSYM group_add_assoc];
      MATCH_ACCEPT_TAC group_add_right_zero]]);;
 
+export_thm group_add_right_cancel_imp;;
+
 (*PARAMETRIC
 let group_add_right_cancel_imp = new_axiom
    `!x y z. group_add y x = group_add z x ==> y = z`;;
@@ -207,6 +217,8 @@ let group_add_right_cancel = prove
     DISCH_THEN SUBST1_TAC THEN
     REFL_TAC]);;
 
+export_thm group_add_right_cancel;;
+
 (*PARAMETRIC
 let group_add_right_cancel = new_axiom
    `!x y z. group_add y x = group_add z x <=> y = z`;;
@@ -218,6 +230,8 @@ let group_add_right_cancel_zero_imp = prove
    MATCH_MP_TAC group_add_right_cancel_imp THEN
    EXISTS_TAC `x : group` THEN
    ASM_REWRITE_TAC [group_add_left_zero]);;
+
+export_thm group_add_right_cancel_zero_imp;;
 
 (*PARAMETRIC
 let group_add_right_cancel_zero_imp = new_axiom
@@ -231,6 +245,8 @@ let group_add_right_cancel_zero = prove
    [MATCH_ACCEPT_TAC group_add_right_cancel_zero_imp;
     DISCH_THEN SUBST1_TAC THEN
     MATCH_ACCEPT_TAC group_add_left_zero]);;
+
+export_thm group_add_right_cancel_zero;;
 
 (*PARAMETRIC
 let group_add_right_cancel_zero = new_axiom
@@ -246,6 +262,8 @@ let group_neg_inj_imp = prove
    POP_ASSUM SUBST1_TAC THEN
    REWRITE_TAC [group_add_left_neg]);;
 
+export_thm group_neg_inj_imp;;
+
 (*PARAMETRIC
 let group_neg_inj_imp = new_axiom
    `!x y. group_neg x = group_neg y ==> x = y`;;
@@ -259,6 +277,8 @@ let group_neg_inj = prove
     DISCH_THEN SUBST1_TAC THEN
     REFL_TAC]);;
 
+export_thm group_neg_inj;;
+
 (*PARAMETRIC
 let group_neg_inj = new_axiom
    `!x y. group_neg x = group_neg y <=> x = y`;;
@@ -269,6 +289,8 @@ let group_neg_zero = prove
    MATCH_MP_TAC group_add_left_cancel_zero_imp THEN
    EXISTS_TAC `group_zero` THEN
    REWRITE_TAC [group_add_right_neg]);;
+
+export_thm group_neg_zero;;
 
 (*PARAMETRIC
 let group_neg_zero = new_axiom
@@ -281,6 +303,8 @@ let group_neg_neg = prove
    MATCH_MP_TAC group_add_left_cancel_imp THEN
    EXISTS_TAC `group_neg x` THEN
    REWRITE_TAC [group_add_left_neg; group_add_right_neg]);;
+
+export_thm group_neg_neg;;
 
 (*PARAMETRIC
 let group_neg_neg = new_axiom
@@ -295,9 +319,39 @@ let group_neg_add = prove
    REWRITE_TAC [group_add_left_neg] THEN
    REWRITE_TAC [group_add_assoc; group_add_left_neg; group_add_left_neg']);;
 
+export_thm group_neg_add;;
+
 (*PARAMETRIC
 let group_neg_add = new_axiom
    `!x y. group_neg (group_add x y) = group_add (group_neg y) (group_neg x)`;;
+*)
+
+let group_neg_left_eq = prove
+  (`!x y. group_add y x = group_zero ==> group_neg x = y`,
+   REPEAT STRIP_TAC THEN
+   MATCH_MP_TAC group_add_right_cancel_imp THEN
+   EXISTS_TAC `x : group` THEN
+   ASM_REWRITE_TAC [group_add_left_neg]);;
+
+export_thm group_neg_left_eq;;
+
+(*PARAMETRIC
+let group_neg_left_eq = new_axiom
+   `!x y. group_add y x = group_zero ==> group_neg x = y`;;
+*)
+
+let group_neg_right_eq = prove
+  (`!x y. group_add x y = group_zero ==> group_neg x = y`,
+   REPEAT STRIP_TAC THEN
+   MATCH_MP_TAC group_add_left_cancel_imp THEN
+   EXISTS_TAC `x : group` THEN
+   ASM_REWRITE_TAC [group_add_right_neg]);;
+
+export_thm group_neg_right_eq;;
+
+(*PARAMETRIC
+let group_neg_right_eq = new_axiom
+   `!x y. group_add x y = group_zero ==> group_neg x = y`;;
 *)
 
 let group_comm_left_neg_imp = prove
@@ -311,6 +365,8 @@ let group_comm_left_neg_imp = prove
    FIRST_X_ASSUM (SUBST1_TAC o SYM) THEN
    REWRITE_TAC
      [GSYM group_add_assoc; group_add_left_neg; group_add_left_zero]);;
+
+export_thm group_comm_left_neg_imp;;
 
 (*PARAMETRIC
 let group_comm_left_neg_imp = new_axiom
@@ -332,6 +388,8 @@ let group_comm_left_neg = prove
     FIRST_ASSUM ACCEPT_TAC;
     MATCH_ACCEPT_TAC group_comm_left_neg_imp]);;
 
+export_thm group_comm_left_neg;;
+
 (*PARAMETRIC
 let group_comm_left_neg = new_axiom
    `!x y.
@@ -348,6 +406,8 @@ let group_comm_right_neg_imp = prove
    CONV_TAC (RAND_CONV (REWR_CONV EQ_SYM_EQ)) THEN
    MATCH_ACCEPT_TAC group_comm_left_neg_imp);;
 
+export_thm group_comm_right_neg_imp;;
+
 (*PARAMETRIC
 let group_comm_right_neg_imp = new_axiom
    `!x y.
@@ -363,6 +423,8 @@ let group_comm_right_neg = prove
    CONV_TAC (LAND_CONV (REWR_CONV EQ_SYM_EQ)) THEN
    CONV_TAC (RAND_CONV (REWR_CONV EQ_SYM_EQ)) THEN
    MATCH_ACCEPT_TAC group_comm_left_neg);;
+
+export_thm group_comm_right_neg;;
 
 (*PARAMETRIC
 let group_comm_right_neg = new_axiom
